src/Div.v
@@ -119,20 +119,24 @@ now destruct Hiq as [|[|]].
 Qed.
 
 Theorem rngl_mul_div_l :
-  rngl_has_inv_and_1_or_divl_or_divr_comm T = true →
+  rngl_has_inv_and_1_comm_or_divl_or_divr_comm T = true →
   ∀ a b : T, a ≠ 0%L → (a * b / a)%L = b.
 Proof.
 intros Hii a b Haz.
-progress unfold rngl_has_inv_and_1_or_divl_or_divr_comm in Hii.
+progress unfold rngl_has_inv_and_1_comm_or_divl_or_divr_comm in Hii.
 apply Bool.orb_true_iff in Hii.
 destruct Hii as [Hii| Hii]. {
   apply Bool.orb_true_iff in Hii.
   destruct Hii as [Hii| Hii]. {
     apply Bool.andb_true_iff in Hii.
+    destruct Hii as (Hii, Hic).
+    apply Bool.andb_true_iff in Hii.
     destruct Hii as (Hiv, Hon).
     progress unfold rngl_div.
     rewrite Hiv.
-...
+    rewrite (rngl_mul_mul_swap Hic).
+    rewrite (rngl_mul_inv_diag_r Hon Hiv); [ | easy ].
+    apply (rngl_mul_1_l Hon).
   } {
     specialize rngl_opt_mul_div_l as H1.
     rewrite Hii in H1.
